Split LLVM into multiple files

LLVMInstructions.thy
@@ -1,91 +1,13 @@
-theory LLVM                                                                                          
-  imports "Word_Lib/Word_64" "Word_Lib/Word_32" "MemoryModel" "RegisterModel"
+theory LLVMInstructions
+  imports "LLVMState"
 begin
-
-section "AST"
-
-
-subsection "Types and values"
-
-datatype llvm_type = i1 | i32 | i64 | f32 | saddr | maddr
-
-datatype llvm_address = saddr memory_model_address | haddr memory_model_address
-
-datatype llvm_value = vi1 bool | vi32 word32 | vi64 word64 | addr llvm_address | poison
-
-type_synonym llvm_memory_model = "llvm_value memory_model"
-type_synonym llvm_register_name = string
-type_synonym llvm_register_model = "(llvm_register_name, llvm_value) register_model"
-
-datatype llvm_value_ref = reg llvm_register_name | val llvm_value
-
-(* Should only have a memory address or memory address... *)
-datatype llvm_pointer = ptr llvm_value_ref
-
-type_synonym llvm_label = string
-
-
-subsection "Instructions"
-
-type_synonym llvm_align = int
-
-datatype llvm_add_wrap = add_nuw | add_nsw | add_nuw_nsw | add_default
-datatype llvm_compare_condition = comp_eq | comp_ne
-                                | comp_ugt | comp_uge | comp_ult | comp_ule
-                                | comp_sgt | comp_sge | comp_slt | comp_sle
-type_synonym llvm_same_sign = bool
-
-
-datatype llvm_instruction = alloca llvm_register_name llvm_type "llvm_align option"
-                          | store llvm_type llvm_value_ref llvm_pointer "llvm_align option"
-                          | load llvm_register_name llvm_type llvm_pointer "llvm_align option"
-                          | add llvm_register_name llvm_add_wrap llvm_type llvm_value_ref llvm_value_ref
-                          | icmp llvm_register_name llvm_same_sign llvm_compare_condition llvm_type llvm_value_ref llvm_value_ref
-                          | phi llvm_register_name llvm_type "(llvm_label * llvm_value_ref) list"
-
-datatype llvm_terminator_instruction = ret llvm_type llvm_value_ref
-                                     | br_i1 llvm_value_ref llvm_label llvm_label
-                                     | br_label llvm_label
-
-
-subsection "Blocks, functions, programs"
-
-type_synonym llvm_instruction_block = "(llvm_instruction list * llvm_terminator_instruction)"
-
-type_synonym llvm_labeled_blocks = "(llvm_label, llvm_instruction_block) mapping"
-
-datatype llvm_block_return = return_value llvm_value
-                           | branch_label llvm_label
-
-datatype llvm_function_definition = func_def string llvm_type
-
-datatype llvm_function = func llvm_function_definition llvm_instruction_block llvm_labeled_blocks
-
-datatype llvm_metadata = meta string string string
-
-type_synonym llvm_attributes = "string list"
-
-datatype llvm_program = program llvm_metadata "llvm_function list" llvm_attributes
 
 
 
 section "Execution"
 
 
-subsection "State"
-
-type_synonym state = "llvm_register_model * llvm_memory_model * llvm_memory_model"
-
-definition empty_state :: "state" where
-  "empty_state = (empty_register_model, empty_memory_model, empty_memory_model)"
-
-definition get_value :: "llvm_register_model \<Rightarrow> llvm_value_ref \<Rightarrow> llvm_value result" where
-  "get_value r v = (case v of (val va) \<Rightarrow> ok va | (reg re) \<Rightarrow> get_register r re)"
-
-
-
-
-subsection "Store instruction helpers"
+subsection "Memory instruction helpers"
 
 fun store_to_stack_or_heap :: "state \<Rightarrow> llvm_address \<Rightarrow> llvm_value \<Rightarrow> state result" where
   "store_to_stack_or_heap (r, s, h) (saddr a) v = do {
@@ -105,12 +27,6 @@ fun store_value :: "state \<Rightarrow> llvm_value_ref \<Rightarrow> llvm_pointe
     store_to_stack_or_heap (r, s, m) ad val
   }"
 
-definition abs_memory :: "state \<Rightarrow> llvm_address \<Rightarrow> llvm_value option option" where
-  "abs_memory = undefined"
-
-definition abs_value :: "state \<Rightarrow> llvm_value_ref \<Rightarrow> llvm_value option" where
-  "abs_value = undefined"
-
 lemma store_value_ok_if[wp_intro]:
   assumes "(\<exists>a ad val s' p. pointer = ptr p \<and> get_value r p = ok a \<and> a = addr ad \<and> get_value r v = ok val \<and> store_to_stack_or_heap (r, s, m) ad val = ok s')"
   shows "(\<exists>s'. store_value (r, s, m) v pointer = ok s')"
@@ -122,31 +38,16 @@ lemma store_value_intro:
   shows "wp_never_err (store_value s v p) Q"
   using assms by auto
 
-lemma store_value_abs:
-  assumes "abs_value s vr = Some v"
-  assumes "abs_value s pr = Some (addr a)"
-  assumes "abs_memory s a \<noteq> None"
-  shows "wp_never_err (store_value s vr p) (\<lambda>s'. abs_value s' = abs_value s \<and> abs_memory s' = (abs_memory s)(a := Some (Some v)))"
-  sorry
 
-lemmas [wp_intro] = store_value_abs[THEN consequence]
-
-thm exE
-
-
-subsection "Load instruction helpers"
-
-
-
-fun load_from_stack_or_heap :: "llvm_memory_model \<Rightarrow> llvm_memory_model \<Rightarrow> llvm_address \<Rightarrow> llvm_value result" where
-  "load_from_stack_or_heap s h (saddr a) = get_memory s a"
-| "load_from_stack_or_heap s h (haddr a) = get_memory h a"
+fun load_from_stack_or_heap :: "state \<Rightarrow> llvm_address \<Rightarrow> llvm_value result" where
+  "load_from_stack_or_heap (r, s, h) (saddr a) = get_memory s a"
+| "load_from_stack_or_heap (r, s, h) (haddr a) = get_memory h a"
 
 fun load_value :: "state \<Rightarrow> llvm_register_name \<Rightarrow> llvm_pointer \<Rightarrow> state result" where
   "load_value (r, s, h) n (ptr p) = do {
     a \<leftarrow> get_value r p;
     ad \<leftarrow> (case a of (addr a') \<Rightarrow> ok a' | _ \<Rightarrow> err not_an_address);
-    v \<leftarrow> load_from_stack_or_heap s h ad;
+    v \<leftarrow> load_from_stack_or_heap (r, s, h) ad;
     r' \<leftarrow> set_register r n v;
     return (r', s, h)
   }"
