LLVMState.thy
@@ -1,0 +1,29 @@
+theory LLVMState
+  imports "LLVMAST" "RegisterModel" "MemoryModel"
+begin
+
+type_synonym state = "llvm_register_model * llvm_memory_model * llvm_memory_model"
+
+definition abs_memory :: "state \<Rightarrow> llvm_address \<Rightarrow> llvm_value option option" where
+  "abs_memory = undefined"
+
+definition abs_value :: "state \<Rightarrow> llvm_value_ref \<Rightarrow> llvm_value option" where
+  "abs_value = undefined"
+
+
+lemma store_value_abs:
+  assumes "abs_value s vr = Some v"
+  assumes "abs_value s pr = Some (addr a)"
+  assumes "abs_memory s a \<noteq> None"
+  shows "wp_never_err (store_value s vr p) (\<lambda>s'. abs_value s' = abs_value s \<and> abs_memory s' = (abs_memory s)(a := Some (Some v)))"
+  sorry
+
+lemmas [wp_intro] = store_value_abs[THEN consequence]
+
+definition empty_state :: "state" where
+  "empty_state = (empty_register_model, empty_memory_model, empty_memory_model)"
+
+definition get_value :: "llvm_register_model \<Rightarrow> llvm_value_ref \<Rightarrow> llvm_value result" where
+  "get_value r v = (case v of (val va) \<Rightarrow> ok va | (reg re) \<Rightarrow> get_register r re)"
+
+end
